typeArith/ocaml/src/eval.ml
@@ -3,28 +3,17 @@ type bool =
 | True
 | False
 
-type term =
-| Tru
-| Fls
-| If of term * term * term
-| O
-| Succ of term
-| Pred of term
-| Iszero of term
-
-(** val natValue : term -> bool **)
-
-let rec natValue = function
-| O -> True
-| Succ t1 -> natValue t1
-| _ -> False
-
-(** val value : term -> bool **)
-
-let value t0 = match t0 with
-| Tru -> True
-| Fls -> True
-| _ -> natValue t0
+module ArithNat =
+ struct
+  type term =
+  | Tru
+  | Fls
+  | If of term * term * term
+  | O
+  | Coq_succ of term
+  | Coq_pred of term
+  | Coq_iszero of term
+ end
 
 type t =
 | Bool
@@ -45,10 +34,10 @@ let eqT t1 t2 =
             | Bool -> False
             | Nat -> True)
 
-(** val has_type : term -> optionT **)
+(** val has_type : ArithNat.term -> optionT **)
 
 let rec has_type = function
-| If (t1, t2, t3) ->
+| ArithNat.If (t1, t2, t3) ->
   (match has_type t1 with
    | SomeT t4 ->
      (match t4 with
@@ -56,25 +45,28 @@ let rec has_type = function
         (match has_type t2 with
          | SomeT t5 ->
            (match has_type t3 with
-            | SomeT t6 -> (match eqT t5 t6 with
-                           | True -> SomeT t5
-                           | False -> NoneT)
+            | SomeT t6 ->
+              (match eqT t5 t6 with
+               | True -> SomeT t5
+               | False -> NoneT)
             | NoneT -> NoneT)
          | NoneT -> NoneT)
       | Nat -> NoneT)
    | NoneT -> NoneT)
-| O -> SomeT Nat
-| Succ t1 -> (match has_type t1 with
-              | SomeT t2 -> (match t2 with
-                             | Bool -> NoneT
-                             | Nat -> SomeT Nat)
-              | NoneT -> NoneT)
-| Pred t1 -> (match has_type t1 with
-              | SomeT t2 -> (match t2 with
-                             | Bool -> NoneT
-                             | Nat -> SomeT Nat)
-              | NoneT -> NoneT)
-| Iszero t1 ->
+| ArithNat.O -> SomeT Nat
+| ArithNat.Coq_succ t1 ->
+  (match has_type t1 with
+   | SomeT t2 -> (match t2 with
+                  | Bool -> NoneT
+                  | Nat -> SomeT Nat)
+   | NoneT -> NoneT)
+| ArithNat.Coq_pred t1 ->
+  (match has_type t1 with
+   | SomeT t2 -> (match t2 with
+                  | Bool -> NoneT
+                  | Nat -> SomeT Nat)
+   | NoneT -> NoneT)
+| ArithNat.Coq_iszero t1 ->
   (match has_type t1 with
    | SomeT t2 -> (match t2 with
                   | Bool -> NoneT
@@ -83,43 +75,64 @@ let rec has_type = function
 | _ -> SomeT Bool
 
 type optiont =
-| Some of term
+| Some of ArithNat.term
 | None
 
-(** val eval : term -> optiont **)
+(** val nVb : ArithNat.term -> bool **)
+
+let rec nVb = function
+| ArithNat.O -> True
+| ArithNat.Coq_succ t1 -> nVb t1
+| _ -> False
+
+(** val vb : ArithNat.term -> bool **)
+
+let vb t0 = match t0 with
+| ArithNat.Tru -> True
+| ArithNat.Fls -> True
+| _ -> nVb t0
+
+(** val eval : ArithNat.term -> optiont **)
 
 let rec eval = function
-| If (t1, t2, t3) ->
-  (match value t1 with
-   | True -> (match t1 with
-              | Tru -> Some t2
-              | Fls -> Some t3
-              | _ -> None)
-   | False -> (match eval t1 with
-               | Some t1' -> Some (If (t1', t2, t3))
-               | None -> None))
-| Succ t1 ->
-  (match natValue t1 with
+| ArithNat.If (t1, t2, t3) ->
+  (match vb t1 with
+   | True ->
+     (match t1 with
+      | ArithNat.Tru -> Some t2
+      | ArithNat.Fls -> Some t3
+      | _ -> None)
+   | False ->
+     (match eval t1 with
+      | Some t1' -> Some (ArithNat.If (t1', t2, t3))
+      | None -> None))
+| ArithNat.Coq_succ t1 ->
+  (match nVb t1 with
    | True -> None
-   | False -> (match eval t1 with
-               | Some t1' -> Some (Succ t1')
-               | None -> None))
-| Pred t1 ->
-  (match natValue t1 with
-   | True -> (match t1 with
-              | O -> Some O
-              | Succ nv1 -> Some nv1
-              | _ -> None)
-   | False -> (match eval t1 with
-               | Some t1' -> Some (Pred t1')
-               | None -> None))
-| Iszero t1 ->
-  (match natValue t1 with
-   | True -> (match t1 with
-              | O -> Some Tru
-              | Succ _ -> Some Fls
-              | _ -> None)
-   | False -> (match eval t1 with
-               | Some t1' -> Some (Iszero t1')
-               | None -> None))
+   | False ->
+     (match eval t1 with
+      | Some t1' -> Some (ArithNat.Coq_succ t1')
+      | None -> None))
+| ArithNat.Coq_pred t1 ->
+  (match nVb t1 with
+   | True ->
+     (match t1 with
+      | ArithNat.O -> Some ArithNat.O
+      | ArithNat.Coq_succ nv1 -> Some nv1
+      | _ -> None)
+   | False ->
+     (match eval t1 with
+      | Some t1' -> Some (ArithNat.Coq_pred t1')
+      | None -> None))
+| ArithNat.Coq_iszero t1 ->
+  (match nVb t1 with
+   | True ->
+     (match t1 with
+      | ArithNat.O -> Some ArithNat.Tru
+      | ArithNat.Coq_succ _ -> Some ArithNat.Fls
+      | _ -> None)
+   | False ->
+     (match eval t1 with
+      | Some t1' -> Some (ArithNat.Coq_iszero t1')
+      | None -> None))
 | _ -> None
