typeArith/ocaml/src/eval.mli
@@ -3,18 +3,17 @@ type bool =
 | True
 | False
 
-type term =
-| Tru
-| Fls
-| If of term * term * term
-| O
-| Succ of term
-| Pred of term
-| Iszero of term
-
-val natValue : term -> bool
-
-val value : term -> bool
+module ArithNat :
+ sig
+  type term =
+  | Tru
+  | Fls
+  | If of term * term * term
+  | O
+  | Coq_succ of term
+  | Coq_pred of term
+  | Coq_iszero of term
+ end
 
 type t =
 | Bool
@@ -26,10 +25,14 @@ type optionT =
 
 val eqT : t -> t -> bool
 
-val has_type : term -> optionT
+val has_type : ArithNat.term -> optionT
 
 type optiont =
-| Some of term
+| Some of ArithNat.term
 | None
 
-val eval : term -> optiont
+val nVb : ArithNat.term -> bool
+
+val vb : ArithNat.term -> bool
+
+val eval : ArithNat.term -> optiont
