typeArith/ocaml/src/print.ml
@@ -1,14 +1,14 @@
 open Eval
 
-let rec eval_string t =
+let rec eval_string (t: ArithNat.term) =
   match t with
   | Tru -> "Tru"
   | Fls -> "Fls"
   | If (t1, t2, t3) -> "If " ^ (eval_string t1) ^ " THEN " ^ (eval_string t2) ^ " ELSE " ^ (eval_string t3)
   | O   -> "0"
-  | Succ t1 -> "S (" ^ (eval_string t1) ^ ")"
-  | Pred t1 -> "Pred " ^ (eval_string t1)
-  | Iszero t1 -> "Is0 " ^ (eval_string t1)
+  | Coq_succ t1 -> "S (" ^ (eval_string t1) ^ ")"
+  | Coq_pred t1 -> "Pred " ^ (eval_string t1)
+  | Coq_iszero t1 -> "Is0 " ^ (eval_string t1)
 
 
 let rec manyeval t1 =
