typeArith/chap8.v
@@ -1,34 +1,12 @@
 Require Coq.extraction.Extraction.
 Extraction Language OCaml.
-
-
-Inductive term : Type :=
-| Tru
-| Fls
-| If (t1 t2 t3: term)
-| O
-| Succ (t1: term)
-| Pred (t1: term)
-| iszero (t1: term).
-
-Fixpoint NatValue (t: term) : bool :=
-  match t with
-  | O => true
-  | Succ t1 => NatValue t1
-  | _ => false
-  end.
-
-Definition Value (t: term) : bool :=
-  match t with
-  | Tru => true
-  | Fls => true
-  | _ => NatValue t
-  end.
+Add LoadPath "../arith/".
+Require Import chap3.
+Import ArithNat.
 
 Inductive T : Type :=
 | Bool
 | Nat.
-
 
 Inductive hastype : term -> T -> Prop :=
 | T_True : hastype Tru Bool
@@ -42,11 +20,11 @@ Inductive hastype : term -> T -> Prop :=
 | T_Succ :
     forall (t1: term),
       hastype t1 Nat ->
-      hastype (Succ t1) Nat
+      hastype (succ t1) Nat
 | T_Pred :
     forall (t1: term),
       hastype t1 Nat ->
-      hastype (Pred t1) Nat
+      hastype (pred t1) Nat
 | T_IsZero :
     forall (t1: term),
       hastype t1 Nat ->
@@ -83,12 +61,12 @@ Fixpoint has_type (t: term) : optionT :=
     | _ => NoneT
     end
   | O => SomeT Nat
-  | Succ t1 =>
+  | succ t1 =>
     match has_type t1 with
     | SomeT Nat => SomeT Nat
     | _ => NoneT
     end
-  | Pred t1 =>
+  | pred t1 =>
     match has_type t1 with
     | SomeT Nat => SomeT Nat
     | _ => NoneT
@@ -157,12 +135,17 @@ Theorem t8_2_4 : forall t R1 R2,
 Proof. intros. induction H; inversion H0; auto. Qed.
 
 Lemma l8_3_1_1 : forall v ,
-    Value v = true -> v \in Bool -> v = Tru \/ v = Fls.
-Proof. intros. inversion H0; subst; auto; inversion H. Qed.
+    value v -> v \in Bool -> v = Tru \/ v = Fls.
+Proof. intros. inversion H0; subst; auto; inversion H. inversion H4. inversion H2. Qed.
 
 Lemma l8_3_1_2 : forall v,
-    Value v = true -> v \in Nat -> NatValue v = true.
-Proof. intros. inversion H0; subst; auto. Qed.
+    value v -> v \in Nat -> NatValue v .
+Proof.
+  intros. inversion H0; subst; auto.
+  inversion H. inversion H4.
+  apply nv_O. inversion H. inversion H2; subst. apply nv_S; auto.
+  inversion H. inversion H2.
+Qed.
 
 Reserved Notation " t '-->' t' " (at level 40).
 Inductive step: term -> term -> Prop :=
@@ -174,17 +157,17 @@ Inductive step: term -> term -> Prop :=
     t1 --> t1' ->
     If t1 t2 t3 --> If t1' t2 t3
 | E_Succ : forall t1 t1',
-    t1 --> t1' -> Succ t1 --> Succ t1'
+    t1 --> t1' -> succ t1 --> succ t1'
 | E_PredZero :
-    Pred O --> O
+    pred O --> O
 | E_PredSucc : forall nv1,
-    NatValue nv1 = true -> Pred (Succ nv1) --> nv1
+    NatValue nv1 -> pred (succ nv1) --> nv1
 | E_Pred : forall t1 t1',
-    t1 --> t1' -> Pred t1 --> Pred t1'
+    t1 --> t1' -> pred t1 --> pred t1'
 | E_IsZeroZero :
     iszero O --> Tru
 | E_IsZeroSucc : forall nv1,
-    NatValue nv1 = true -> iszero (Succ nv1) --> Fls
+    NatValue nv1 -> iszero (succ nv1) --> Fls
 | E_IsZero : forall t1 t1',
     t1 --> t1' -> iszero t1 --> iszero t1'
 
@@ -194,10 +177,24 @@ Inductive optiont : Type :=
 | Some (T: term)
 | None.
 
+Fixpoint NVb (t: term) : bool :=
+  match t with
+  | O => true
+  | succ t1 => NVb t1
+  | _ => false
+  end.
+
+Definition Vb (t: term) : bool :=
+  match t with
+  | Tru => true
+  | Fls => true
+  | _ => NVb t
+  end.
+
 Fixpoint eval (t: term) : optiont :=
   match t with
   | If t1 t2 t3 =>
-    if (Value t1) then
+    if (Vb t1) then
       match t1 with
       | Tru => Some t2
       | Fls => Some t3
@@ -207,29 +204,29 @@ Fixpoint eval (t: term) : optiont :=
       | Some t1' => Some (If t1' t2 t3)
       | _ => None
       end
-  | Succ t1 =>
-    if NatValue t1 then
+  | succ t1 =>
+    if NVb t1 then
       None else
       match (eval t1) with
-      | Some t1' => Some (Succ t1')
+      | Some t1' => Some (succ t1')
       | _ => None
       end
-  | Pred t1 =>
-    if (NatValue t1) then
+  | pred t1 =>
+    if (NVb t1) then
       match t1 with
       | O => Some O
-      | Succ nv1 => Some nv1
+      | succ nv1 => Some nv1
       | _ => None
       end else
       match (eval t1) with
-      | Some t1' => Some (Pred t1')
+      | Some t1' => Some (pred t1')
       | _ => None
       end
   | iszero t1 =>
-    if (NatValue t1) then
+    if (NVb t1) then
       match t1 with
       | O => Some Tru
-      | Succ _ => Some Fls
+      | succ _ => Some Fls
       | _ => None
       end else
       match (eval t1) with
@@ -252,14 +249,25 @@ Ltac solve_by_invert :=
 
 
 Lemma Valuestop : forall t1,
-    Value t1 = true -> not (exists t1', t1 --> t1').
+    Vb t1 = true -> not (exists t1', t1 --> t1').
 Proof.
   induction t1; intros; intro H1; try solve_by_inverts 2.
   inversion H.
-  assert (Value t1 = true). destruct t1; try solve_by_invert; auto.
+  assert (Vb t1 = true). destruct t1; try solve_by_invert; auto.
   apply IHt1 in H0. inversion H1. inversion H3; subst. induction H0. exists t1'; auto.
 Qed.
 
+
+Lemma NVb_correct : forall t,
+    NatValue t <-> NVb t = true.
+Proof.
+  split; intros.
+  -
+    induction H; auto.
+  -
+    induction t; try solve_by_invert; auto.
+    apply nv_O. inversion H. apply nv_S; auto.
+Qed.
 
 Theorem step_eval1_correct : forall t1 t1',
     eval t1 = Some t1' <-> t1 --> t1'.
@@ -269,61 +277,72 @@ Proof.
     intros. generalize dependent t1'.
     induction t1; intros; try solve_by_invert.
     +
-      inversion H. destruct (Value t1_1). destruct (t1_1); try solve_by_invert.
+      inversion H. destruct (Vb t1_1). destruct (t1_1); try solve_by_invert.
       inversion H. apply E_IfTrue. inversion H. apply E_IfFalse.
       destruct (eval t1_1); try solve_by_invert. inversion H1. apply E_If. apply IHt1_1; auto.
     +
-      inversion H. destruct (NatValue t1). inversion H1. destruct (eval t1). inversion H1. apply E_Succ. apply IHt1; auto. inversion H1.
+      inversion H. destruct (NVb t1). inversion H1. destruct (eval t1). inversion H1. apply E_Succ. apply IHt1; auto. inversion H1.
     +
-      inversion H. destruct (NatValue t1) eqn:nv. destruct (t1); try (solve_by_invert). inversion H1. apply E_PredZero.
-      inversion H1. apply E_PredSucc. inversion nv. rewrite H2; auto.
+      inversion H. destruct (NVb t1) eqn:nv. destruct (t1); try (solve_by_invert). inversion H1. apply E_PredZero.
+      inversion H1. apply E_PredSucc. inversion nv. rewrite <- H2. apply NVb_correct; auto.
       destruct (eval t1). inversion H1. apply E_Pred. apply IHt1; auto.
       inversion H1.
     +
-      inversion H. destruct (NatValue t1) eqn:nv. destruct t1; try solve_by_invert.
-      inversion H1. apply E_IsZeroZero. inversion H1. apply E_IsZeroSucc. inversion nv. auto.
+      inversion H. destruct (NVb t1) eqn:nv. destruct t1; try solve_by_invert.
+      inversion H1. apply E_IsZeroZero. inversion H1. apply E_IsZeroSucc. inversion nv. apply NVb_correct; auto.
       destruct (eval t1). inversion H1. apply E_IsZero. apply IHt1; auto. inversion H1.
 
   -
     generalize dependent t1'; induction t1; intros; try (solve_by_invert).
     +
       inversion H; subst; auto.
-      simpl. destruct (Value t1_1) eqn:Ht1. induction Valuestop with(t1:= t1_1); auto. eauto.
+      simpl. destruct (Vb t1_1) eqn:Ht1. induction Valuestop with(t1:= t1_1); auto. eauto.
       apply IHt1_1 in H4. rewrite H4; auto.
     +
-      simpl. inversion H; subst. destruct (NatValue t1) eqn:nv.
+      simpl. inversion H; subst. destruct (NVb t1) eqn:nv.
       induction (Valuestop t1). destruct (t1); try solve_by_invert; auto. eauto.
       apply IHt1 in H1. rewrite H1; auto.
     +
-      inversion H; subst; auto. simpl. rewrite H1; auto.
-      simpl. destruct (NatValue t1) eqn:nv. induction (Valuestop t1). destruct t1; try solve_by_invert.
+      inversion H; subst; auto. simpl. apply NVb_correct in H1. rewrite H1; auto.
+      simpl. destruct (NVb t1) eqn:nv. induction (Valuestop t1). destruct t1; try solve_by_invert.
       simpl. inversion nv; auto. eauto.
       apply IHt1 in H1. rewrite H1; auto.
     +
-      inversion H; subst; auto. simpl. rewrite H1; auto.
-      simpl. destruct (NatValue t1) eqn:nv. induction (Valuestop t1). destruct t1; try solve_by_invert; eauto. eauto.
+      inversion H; subst; auto. simpl. apply NVb_correct in H1. rewrite H1; auto.
+      simpl. destruct (NVb t1) eqn:nv. induction (Valuestop t1). destruct t1; try solve_by_invert; eauto. eauto.
       apply IHt1 in H1. rewrite H1; auto.
 Qed.
 
 Extraction "ocaml/src/eval.ml" eval has_type.
 
+Lemma Vb_correct : forall t,
+    value t <-> Vb t = true.
+Proof with eauto.
+  split; intros.
+  -
+    induction H; auto. inversion H. auto. simpl. apply NVb_correct; auto.
+  -
+    induction t; try solve_by_invert; auto. apply v_tru. apply v_fls.
+    apply v_nat. apply nv_O. apply v_nat. inversion H. apply nv_S; apply NVb_correct; auto.
+Qed.
+
 Theorem l8_3_2 : forall t T',
-    t \in T' -> Value t = true \/ exists t', t --> t'.
+    t \in T' -> Vb t = true \/ exists t', t --> t'.
 Proof with eauto.
   induction t; intros; auto.
   - (*If*)
     inversion H. inversion H0; subst. generalize H3. right. apply IHt1 in H3.
-    inversion H3. apply l8_3_1_1 in H0; auto. inversion H0; subst. exists t2. apply E_IfTrue. exists t3; apply E_IfFalse.
+    inversion H3. apply l8_3_1_1 in H0; auto. inversion H0; subst. exists t2. apply E_IfTrue. exists t3; apply E_IfFalse. apply Vb_correct; auto.
     inversion H1. exists (If x t2 t3). apply E_If; auto.
   - (*Succ*)
-    inversion H; subst. generalize H1. apply IHt in H1. inversion H1. left. apply l8_3_1_2 in H2; auto.
-    inversion H0. right. exists (Succ x). apply E_Succ...
+    inversion H; subst. generalize H1. apply IHt in H1. inversion H1. left. apply l8_3_1_2 in H2; auto. simpl. apply NVb_correct; auto. apply Vb_correct...
+    inversion H0. right. exists (succ x). apply E_Succ...
   - (*Pred*)
-    inversion H; subst. generalize H1. right. apply IHt in H1. inversion H1. apply l8_3_1_2 in H2...
-    destruct t; inversion H2. exists O. apply E_PredZero. exists t. apply E_PredSucc... inversion H2. exists (Pred x). apply E_Pred...
+    inversion H; subst. generalize H1. right. apply IHt in H1. inversion H1. apply Vb_correct in H2. apply l8_3_1_2 in H2...
+    destruct t; inversion H2. exists O. apply E_PredZero. exists t. apply E_PredSucc... inversion H2. exists (pred x). apply E_Pred...
   - (*iszero*)
     inversion H; subst. generalize H1. right. apply IHt in H1. inversion H1.
-    apply l8_3_1_2 in H0... destruct t; inversion H0. exists Tru. apply E_IsZeroZero. exists Fls. apply E_IsZeroSucc...
+    apply l8_3_1_2 in H0... destruct t; inversion H0. exists Tru. apply E_IsZeroZero. exists Fls. apply E_IsZeroSucc... apply Vb_correct...
     inversion H2. exists (iszero x). apply E_IsZero...
 Qed.
 
@@ -354,26 +373,26 @@ Reserved Notation " t '==>' t' " (at level 40).
 
 Inductive bigstep : term -> term -> Prop :=
 | B_Value : forall t1,
-    Value t1 = true -> t1 ==> t1
+    value t1 -> t1 ==> t1
 | B_IfTrue : forall t1 t2 v2 t3,
-    t1 ==> Tru -> t2 ==> v2 -> Value v2 = true -> If t1 t2 t3 ==> v2
+    t1 ==> Tru -> t2 ==> v2 -> value v2 -> If t1 t2 t3 ==> v2
 | B_IfFalse : forall t1 t2 t3 v3,
-    t1 ==> Fls -> t3 ==> v3 -> Value v3 = true -> If t1 t2 t3 ==> v3
+    t1 ==> Fls -> t3 ==> v3 -> value v3 -> If t1 t2 t3 ==> v3
 | B_Succ : forall t1 nv1,
-    t1 ==> nv1 -> NatValue nv1 = true -> Succ t1 ==> Succ nv1
+    t1 ==> nv1 -> NatValue nv1 -> succ t1 ==> succ nv1
 | B_PredZero : forall t1,
-    t1 ==> O -> Pred t1 ==> O
+    t1 ==> O -> pred t1 ==> O
 | B_PredSucc : forall t1 nv1,
-    t1 ==> (Succ nv1) -> NatValue nv1 = true -> Pred t1 ==> nv1
+    t1 ==> (succ nv1) -> NatValue nv1 -> pred t1 ==> nv1
 | B_IsZeroZero : forall t1,
     t1 ==> O -> iszero t1 ==> Tru
 | B_IsZeroSucc : forall t1 nv1,
-    t1 ==> (Succ nv1) -> NatValue nv1 = true -> iszero t1 ==> Fls
+    t1 ==> (succ nv1) -> NatValue nv1 -> iszero t1 ==> Fls
 
   where " t '==>' t' " := (bigstep t t').
 
 Lemma NatValueType : forall t1,
-    NatValue t1 = true -> t1 \in Nat.
+    NatValue t1 -> t1 \in Nat.
 Proof. intros. induction t1; inversion H. apply T_Zero. apply T_Succ. apply IHt1. auto. Qed.
 
 Lemma l8_3_7_preservation : forall t t' T,
@@ -381,50 +400,51 @@ Lemma l8_3_7_preservation : forall t t' T,
 Proof with eauto.
   induction t; intros; inversion H. inversion H1; subst... inversion H1; subst...
   -
-    inversion H1; inversion H0; subst. inversion H2. apply IHt2... apply IHt3...
+    inversion H1; inversion H0; subst. inversion H2. inversion H3. apply IHt2... apply IHt3...
   -
     inversion H1...
   -
     inversion H1; subst... inversion H0; subst. apply T_Succ. apply IHt...
   -
-    inversion H0; inversion H1; subst. inversion H5. apply T_Zero. apply NatValueType...
+    inversion H0; inversion H1; subst. inversion H5. inversion H2. apply T_Zero. apply NatValueType...
   -
     inversion H0; inversion H1; subst... apply T_True. apply T_False.
 Qed.
 
 Lemma l8_3_7_progress : forall t T',
-    t \in T' -> (exists t', t ==> t' /\ Value t' = true).
+    t \in T' -> (exists t', t ==> t' /\ Vb t' = true).
 Proof with eauto.
   induction t; intros.
   -
-    exists Tru; split... apply B_Value...
+    exists Tru; split... apply B_Value... apply v_tru.
   -
-    exists Fls; split... apply B_Value...
+    exists Fls; split... apply B_Value... apply v_fls.
   -
     inversion H; subst. generalize H3. intros. apply IHt1 in H3. inversion H3. inversion H1.
     assert (x \in Bool). eapply l8_3_7_preservation. split. apply H0. apply H2.
     apply l8_3_1_1 in H7... inversion H7.
-    apply IHt2 in H5. inversion H5. inversion H9. exists x0. subst. split. apply B_IfTrue... apply H11.
-    apply IHt3 in H6; inversion H6. inversion H9. exists x0; subst. split... apply B_IfFalse...
+    apply IHt2 in H5. inversion H5. inversion H9. exists x0. subst. split. apply B_IfTrue... apply Vb_correct; auto. apply H11.
+    apply IHt3 in H6; inversion H6. inversion H9. exists x0; subst. split... apply B_IfFalse... apply Vb_correct; apply H11. apply Vb_correct; apply H4.
   -
-    exists O. split... apply B_Value...
+    exists O. split... apply B_Value... apply v_nat. apply nv_O.
   -
-    inversion H;subst. generalize H1. apply IHt in H1. inversion H1. inversion H0. exists (Succ x).
-    apply l8_3_1_2 in H3; auto.
-    split. apply B_Succ... auto. apply l8_3_7_preservation with (t:= t). split...
+    inversion H;subst. generalize H1. apply IHt in H1. inversion H1. inversion H0. exists (succ x).
+    apply Vb_correct in H3. apply l8_3_1_2 in H3; auto.
+    split. apply B_Succ... simpl. apply NVb_correct; auto.
+    apply l8_3_7_preservation with (t:= t). split...
   -
     inversion H; subst. generalize H1. apply IHt in H1. inversion H1. inversion H0. intro.
-    apply l8_3_1_2 in H3. destruct x; inversion H3. exists O. split. apply B_PredZero... auto.
-    exists x. split... apply B_PredSucc... generalize H6. clear. induction x; intros H; inversion H...
+    apply Vb_correct in H3. apply l8_3_1_2 in H3. destruct x; inversion H3. exists O. split. apply B_PredZero... auto.
+    exists x. split... apply B_PredSucc... apply Vb_correct. apply v_nat; auto. 
     apply l8_3_7_preservation with (t:= t)...
   -
     inversion H; subst. generalize H1. apply IHt in H1. inversion H1. inversion H0. intro.
-    apply l8_3_1_2 in H3. destruct x; inversion H3. exists Tru. split... apply B_IsZeroZero...
+    apply Vb_correct in H3. apply l8_3_1_2 in H3. destruct x; inversion H3. exists Tru. split... apply B_IsZeroZero...
     exists Fls. split... apply B_IsZeroSucc with (nv1:= x)... apply l8_3_7_preservation with (t:= t)...
 Qed.
 
 Definition stop (t1: term) :=
-  Value t1 = false  /\ not (exists t1', t1 --> t1').
+  Vb t1 = false  /\ not (exists t1', t1 --> t1').
 
 Theorem has_typeStop: forall t,
     stop t -> has_type t = NoneT.
@@ -438,11 +458,11 @@ Proof with eauto.
     apply l8_3_2 in H0. inversion H0. inversion H1. auto.
   -
     simpl. destruct (has_type t) eqn:Ht... destruct T1... induction H0.
-    assert (Succ t \in Nat). apply has_typeCorrect. simpl. rewrite Ht...
+    assert (succ t \in Nat). apply has_typeCorrect. simpl. rewrite Ht...
     apply l8_3_2 in H0. inversion H0. rewrite H1 in H. discriminate. auto.
   -
     simpl. destruct (has_type t) eqn:Ht... destruct T1... induction H0.
-    assert (Pred t \in Nat). apply has_typeCorrect. simpl. rewrite Ht...
+    assert (pred t \in Nat). apply has_typeCorrect. simpl. rewrite Ht...
     apply l8_3_2 in H0. inversion H0. discriminate. auto.
   -
     simpl. destruct (has_type t) eqn:Ht... destruct T1... induction H0.
